Plfl/DeBruijn.lean
@@ -1,0 +1,56 @@
+inductive Ty : Type
+  | bool : Ty
+  | arr : Ty → Ty → Ty
+
+notation "bool" => Ty.bool
+notation:70 τ₁ "⇒" τ₂ => Ty.arr τ₁ τ₂
+
+inductive Context : Type
+  | empty : Context
+  | cons : Context → Ty → Context
+
+notation "∅" => Context.empty
+notation:50 Γ ";" τ => Context.cons Γ τ
+
+inductive Lookup : Context → Ty → Prop
+  | here {Γ τ} : Lookup (Γ ; τ) τ
+  | there {Γ τ τ'} : Lookup Γ τ → Lookup (Γ ; τ') τ
+
+notation:40 Γ "∋" τ:40 => Lookup Γ τ
+
+inductive Judgement : Context → Ty → Type
+  | var {Γ τ} : Γ ∋ τ → Judgement Γ τ
+  | app {Γ τ τ'} : Judgement Γ (τ ⇒ τ') → Judgement Γ τ → Judgement Γ τ'
+  | lam {Γ τ τ'} : Judgement (Γ ; τ) τ' → Judgement Γ (τ ⇒ τ')
+  | tru {Γ} : Judgement Γ bool
+  | fls {Γ} : Judgement Γ bool
+  | ite {Γ τ} : Judgement Γ bool → Judgement Γ τ → Judgement Γ τ → Judgement Γ τ
+
+notation:40 Γ "⊢" τ:40 => Judgement Γ τ
+notation "true"  => Judgement.tru
+notation "false" => Judgement.fls
+prefix:90 "$ "   => Judgement.var
+notation:50 "λ" t:50 => Judgement.lam t
+infix:70 " ⬝ "   => Judgement.app
+notation "if" c "then" t₁ "else" t₂ => Judgement.ite c t₁ t₂
+
+def length : Context → Nat
+  | Context.empty => 0
+  | Context.cons Γ _ => length Γ + 1
+
+def lookup : ∀ {Γ : Context} {n : Nat}, (h : n < length Γ) → Ty
+  | Context.cons _ τ,     0, _ => τ
+  | Context.cons _ _, _ + 1, h => lookup (Nat.lt_of_succ_lt h)
+
+def count : ∀ {Γ : Context} {n : Nat}, (h : n < length Γ) → Γ ∋ lookup h
+  | Context.cons _ τ,     0, _ => Lookup.here
+  | Context.cons _ _, _ + 1, h => Lookup.there (count (Nat.lt_of_succ_lt h))
+/-
+def ex : ∅ ⊢ (bool ⇒ bool) ⇒ bool ⇒ bool
+  := λ λ (ref 1 · (ref 1 · ref 0))
+-/
+
+def ref {Γ : Context} : (n : Nat) → (h : n + 1 < length Γ) → Γ ∋ lookup h
+  | _ , h => count h
+
+def ex : ∅ ⊢ (bool ⇒ bool) ⇒ bool ⇒ bool := by sorry
