Plfl/STLCProp.lean
@@ -10,7 +10,7 @@ import Plfl.STLC
   3. t = λx:τ'.t'
 -/
 theorem canonical_forms_bool
-  : ∀ t, (∅ ⊢ t : bool) → Val t → t = true ∨ t = false
+  : ∀ t, ∅ ⊢ t : bool → Val t → t = true ∨ t = false
   := by
     intros t ht hv
     cases hv with
@@ -19,7 +19,7 @@ theorem canonical_forms_bool
     | lam => cases ht
 
 theorem canonical_forms_lam
-  : ∀ t τ₁ τ₂, (∅ ⊢ t : τ₁ ⇒ τ₂) → Val t → ∃ x t', t = (λ x : τ₁ ⇒ t')
+  : ∀ t τ₁ τ₂, ∅ ⊢ t : τ₁ ⇒ τ₂ → Val t → ∃ x t', t = λ x : τ₁ ⇒ t'
   := by
     intros t τ₁ τ₂ ht hv
     cases hv with
@@ -34,42 +34,49 @@ theorem canonical_forms_lam
 /- Theorem progress : ∀ t T,
   empty |-- t \in T →
   value t ∨ ∃ t', t --> t'. -/
+def progress_measure : Tm → Nat
+  | Tm.var _ => 1
+  | Tm.app t₁ t₂ => progress_measure t₁ + progress_measure t₂ + 1
+  | Tm.lam _ _ t => progress_measure t + 1
+  | Tm.tru => 1
+  | Tm.fls => 1
+  | Tm.ite t₁ t₂ _ => progress_measure t₁ + progress_measure t₂ + 1
 
-theorem progress : ∀ t τ, (∅ ⊢ t : τ) → Val t ∨ (∃ t', t —⟶ t') := by
+theorem progress : ∀ {t τ}, ∅ ⊢ t : τ → Val t ∨ (∃ t', t —⟶ t') := by
   intro t τ ht
   cases ht with
   | var x =>
       apply Or.inl
       contradiction
   | @app _ t₁ t₂ τ₁ _ ht₁ ht₂ =>
-      have ht₁' := progress t₁ (τ₁⇒τ) ht₁
+      have ht₁' := progress ht₁
       cases ht₁' with
       | inl hv₁ =>
-          have ht₂' := progress t₂ τ₁ ht₂
+          have ht₂' := progress ht₂
           cases ht₂' with
           | inl hv₂ =>
               apply Or.inr
               cases hv₁ with
               | @lam x _ t =>
-                  exists (t [x ↦ t₂])
+                  exists t [x ↦ t₂]
                   apply (Reduction.app_abs hv₂)
               | tru => cases ht₁
               | fls => cases ht₁
           | inr hstep₂ =>
               apply Or.inr
               have ⟨t₂', hstep₂'⟩ := hstep₂
-              exists (t₁ ⬝ t₂')
+              exists t₁ ⬝ t₂'
               apply (Reduction.app₂ hv₁ hstep₂')
       | inr hstep₁ =>
           apply Or.inr
           have ⟨t₁', hstep₁'⟩ := hstep₁
-          exists (t₁' ⬝ t₂)
+          exists t₁' ⬝ t₂
           apply (Reduction.app₁ hstep₁')
   | lam ht => apply Or.inl Val.lam
   | tru => apply Or.inl Val.tru
   | fls => apply Or.inl Val.fls
   | @ite _ t₁ t₂ t₃ _ ht₁ ht₂ ht₃ =>
-      have ht₁' := progress t₁ bool ht₁
+      have ht₁' := progress ht₁
       cases ht₁' with
       | inl hv₁ =>
           cases hv₁ with
@@ -80,44 +87,29 @@ theorem progress : ∀ t τ, (∅ ⊢ t : τ) → Val t ∨ (∃ t', t —⟶ t'
           apply Or.inr
           have ⟨t₁', hstep₁'⟩ := hstep₁
           apply (Exists.intro (if t₁' then t₂ else t₃) (Reduction.ite hstep₁'))
-termination_by progress t _ _  => t
+-- termination_by _ t _ _ => progress_measure t
 
 -- Lemma: Weekening
-theorem weakening : ∀ Γ Γ' t τ, (Γ ⊂ Γ') → (Γ ⊢ t : τ) → Γ' ⊢ t : τ := by
-  intro Γ Γ' t τ hsub ht
-  induction ht with
-  | var x =>
-      cases hsub
-      apply Ty.var
-      assumption
-  | app ht₁ ht₂ =>
-      cases hsub
-      apply Ty.app
-      apply ht₁
-      apply ht₂
-  | lam ht =>
-      cases hsub
-      apply Ty.lam
-      apply ht
-  | tru =>
-      cases hsub
-      apply Ty.tru
-  | fls =>
-      cases hsub
-      apply Ty.fls
-  | ite ht₁ ht₂ ht₃ =>
-      cases hsub
-      apply Ty.ite
-      apply ht₁
-      apply ht₂
-      apply ht₃
+theorem weakening : ∀ {Γ t τ}, ∅ ⊢ t : τ → Γ ⊢ t : τ := by
+  intro Γ t τ ht
+  cases ht with
+  | var x => contradiction
+  | @app Γ' t₁ t₂ τ₁ τ₂ ht₁ ht₂ => sorry
+  | lam ht => sorry
+  | tru => apply Judgement.tru
+  | fls => apply Judgement.fls
+  | @ite t₁ t₂ t₃ ht₁ ht₂ ht₃ => sorry
+
+theorem substitution_preseserves
+  : ∀ {Γ x t v τ₁ τ₂}, ∅ ⊢ v : τ₁ → Γ; x : τ₁ ⊢ t : τ₂ → Γ ⊢ t [x ↦ v] : τ₂
+  := sorry
 
 /-
   Theorem: Preservation
 
   If Γ ⊢ t : τ and t —⟶ t', then Γ ⊢ t' : τ.
 -/
-theorem preservation : ∀ t t' τ, (∅ ⊢ t : τ) → (t —⟶ t') → ∅ ⊢ t' : τ := by
+theorem preservation : ∀ t t' τ, ∅ ⊢ t : τ → t —⟶ t' → ∅ ⊢ t' : τ := by
   intro t t' τ ht hstep
   cases ht with
   | var x => cases hstep
